Progress on LtkReduction step

ntor/Security.ec
@@ -4595,6 +4595,7 @@ by case : (tltkr) => />.
   rcondf ^if; auto => />. *)
 qed.
 
+
 (*
 lemma game4_eph &m: Pr[E_GAKE_nodhs(Game4, A).run(true) @ &m : Game4.badq /\ Game4.test_ephrev_s = false] <= 
                   Pr[E_GAKE_nodhs(Game4Eph, A).run(true) @ &m : Game4Eph.badq].
@@ -4602,17 +4603,333 @@ byequiv (: ={glob A, arg} /\ arg{1} = true ==> _) => //.
 proc; inline *.
 call (: Game4Eph.test_ephrev_s
       , ={b0, hm, h1m, h2m, c_smap, s_smap, servers, tested, b_set, x_set, y_set, pk_set, m1_set, m2_set, bad1, bad2, tq, hq, badq, test_ephrev_s, test_ltkrev}(Game4, Game4Eph)
+        /\ Game4.b0{1}
+        /\ (inv_Game4 Game4.tested Game4.tq Game4.badq Game4.pk_set Game4.m1_set Game4.m2_set Game4.x_set Game4.y_set Game4.s_smap Game4.hq Game4.c_smap Game4.h1m Game4.h2m Game4.servers){1}
       , ={test_ephrev_s}(Game4, Game4Eph)
 ) => //; last first.
 
-auto => />.
-move => rl rr al bl b1l b2l bql csl h1ml h2ml hql m1l m2l pkl ssm sm tltkl tl tql xl yl ar br b1r b2r bqr csr h1mr h2mr hqr m1r m2r pkr ssr sr tephr tltkr tr tqr xr yr. 
+auto => |>.
+split; 1: by smt(emptyE in_fset0 in_fsetU).
+move => inv rl rr al bl b1l b2l bql csl h1ml h2ml hql m1l m2l pkl ssm sm tltkl tl tql xl yl ar br b1r b2r bqr csr h1mr h2mr hqr m1r m2r pkr ssr sr tephr tltkr tr tqr xr yr.
 
-auto => />.
+by case (tephr) => //. 
 
 - exact A_ll.
 
-*)
+(* h *)
+- conseq (: ={res} /\ ={b0, hm, h1m, h2m, c_smap, s_smap, servers, tested, b_set, x_set, y_set, pk_set, m1_set, m2_set, bad1, bad2, tq, hq, badq, test_ephrev_s, test_ltkrev}(Game4, Game4Eph)) Game4_inv_h => //.
+  proc; inline.
+  sp; if => //.
+  sp; seq 1 1: (#pre /\ ={t}); 1: by auto => />.
+  if => //.
+  + sp; seq 1 1: (#pre /\ ={k}); 1: by auto => />. 
+    if => //.
+    + auto => />.
+    auto => />.
+  sp; seq 1 1: (#pre /\ ={k}); 1: by auto => />. 
+  if => //.
+  + auto => />.
+  auto => />.
+- move => &2 bad; proc; sp; if; auto => />. 
+  rewrite dkey_ll dtag_ll //=.  
+- move => &1; proc; auto.
+  rcondf ^if; auto => />.
+
+(* init_s *)
+- conseq (: ={res} /\ ={b0, hm, h1m, h2m, c_smap, s_smap, servers, tested, b_set, x_set, y_set, pk_set, m1_set, m2_set, bad1, bad2, tq, hq, badq, test_ephrev_s, test_ltkrev}(Game4, Game4Eph)) Game4_inv_init_s => //.
+  proc.
+  sp; if => //.
+  sp; seq 1 1: (#pre /\ ={sk}); 1: by auto.
+  sp 1 1; if => //.
+  auto => />.
+- move => &2 bad.
+  proc; sp; if; auto => />.
+  rewrite dt_ll //=. 
+- move => &1. 
+  proc. 
+  rcondf ^if; auto => />.
+
+(* send_msg1 *)
+- conseq (: ={res} /\ ={b0, hm, h1m, h2m, c_smap, s_smap, servers, tested, b_set, x_set, y_set, pk_set, m1_set, m2_set, bad1, bad2, tq, hq, badq, test_ephrev_s, test_ltkrev}(Game4, Game4Eph)) Game4_inv_send_msg1 => //.
+  proc.
+  sp; if => //.
+  sp; if => //.
+  sp; match = => //. 
+  seq 1 1: (#pre /\ ={sk}); 1: by auto.
+  auto => />.
+- move => &2 bad.
+  proc; sp; if => //; sp; if. 
+  + match; auto => />.
+    rewrite dt_ll //=.
+  by auto.
+- move => &1. 
+  proc. 
+  rcondf ^if; auto => />.
+
+(* send_msg2 *)
+- conseq (: ={res} /\ ={b0, hm, h1m, h2m, c_smap, s_smap, servers, tested, b_set, x_set, y_set, pk_set, m1_set, m2_set, bad1, bad2, tq, hq, badq, test_ephrev_s, test_ltkrev}(Game4, Game4Eph)) Game4_inv_send_msg2 => //.
+  proc; inline. 
+  sp; if => //.
+  sp; match = => // sko.
+  match = => //.
+  + seq 1 1: (#pre /\ ={sk}); 1: by auto.
+  sp 3 3; if => //. 
+  sp 2 2; seq 1 1: (#pre /\ ={ts}); 1: by auto => />.
+  if => //.
+  + sp 3 3; if => //.
+    + auto => /> &2 *.
+    auto => /> *.
+  sp 2 2; if => //.
+  + auto => /> &2 *.
+  auto => /> *.
+- move => &2 bad.
+  proc; inline; sp; if; sp. 
+  match; auto => />.
+  match; auto => />.
+  seq 1 : (#pre); try by auto.
+  + auto => />. by rewrite dt_ll.
+  + sp; if => //. 
+    auto => />.
+    rewrite dtag_ll //=. 
+  + hoare. 
+    by auto => />.
+  auto => />.
+- move => &1. 
+  proc; inline.
+  rcondf ^if; auto => />.
+
+(* send_msg3 *)
+- conseq (: ={res} /\ ={b0, hm, h1m, h2m, c_smap, s_smap, servers, tested, b_set, x_set, y_set, pk_set, m1_set, m2_set, bad1, bad2, tq, hq, badq, test_ephrev_s, test_ltkrev}(Game4, Game4Eph)) Game4_inv_send_msg3 => //.
+  proc; inline.
+  sp; if => //.
+  sp; match = => // st.
+  match = => // s pt ir.
+  sp; seq 1 1 : (#pre /\ ={ts}); 1: by auto => />.
+  if => //.
+  + auto => /> &2 *.
+  auto => /> &2 *.
+- move => &2 bad.
+  proc; inline.
+  sp; if => //.
+  sp; match; auto. 
+  match => //.
+  sp; seq 1 : (#pre); try by auto.
+  + auto => />. by rewrite dtag_ll.
+  hoare. 
+  by auto => />.
+- move => &1.
+  proc; inline*.
+  rcondf ^if; auto => />.
+
+(* c_rev_skey *)
+- conseq (: ={res} /\ ={b0, hm, h1m, h2m, c_smap, s_smap, servers, tested, b_set, x_set, y_set, pk_set, m1_set, m2_set, bad1, bad2, tq, hq, badq, test_ephrev_s, test_ltkrev}(Game4, Game4Eph)) Game4_inv_c_rev_skey => //.
+  proc; inline.
+  sp; if => //.
+  sp; match = => // st.
+  match = => // s t k ir.
+  if => //.
+  sp; seq 1 1: (#pre /\ ={ks}); 1: by auto => />.
+  if => //.
+  + auto => /> &2 *. 
+  auto => /> &2 *.
+- move => &2 bad.
+  proc; sp; if => //; sp.
+  match => //. 
+  match => //; if.
+  + sp; seq 1 : (#pre); try by auto.
+    + auto => />. by rewrite dkey_ll.
+    hoare. 
+    by auto => />.
+  auto => />.
+- move => &1.
+  proc; inline*.
+  rcondf ^if; auto => />.
+
+(* s_rev_skey *)
+- conseq (: ={res} /\ ={b0, hm, h1m, h2m, c_smap, s_smap, servers, tested, b_set, x_set, y_set, pk_set, m1_set, m2_set, bad1, bad2, tq, hq, badq, test_ephrev_s, test_ltkrev}(Game4, Game4Eph)) Game4_inv_s_rev_skey => //.
+  proc; inline.
+  sp; if => //.
+  sp; match = => // st.
+  match = => // s t k ir.
+  if => //.
+  sp; seq 1 1: (#pre /\ ={ks}); 1: by auto => />.
+  if => //.
+  + auto => /> &2 *.
+  auto => /> &2 *.
+- move => &2 bad.
+  proc; sp; if => //.  
+  match => //. 
+  match => //; if; auto => />.
+  rewrite dkey_ll //=.
+- move => &1.
+  proc; inline*.
+  rcondf ^if; auto => />.
+
+(* rev_ltkey *)
+- conseq (: ={res} /\ ={b0, hm, h1m, h2m, c_smap, s_smap, servers, tested, b_set, x_set, y_set, pk_set, m1_set, m2_set, bad1, bad2, tq, hq, badq, test_ephrev_s, test_ltkrev}(Game4, Game4Eph)) Game4_inv_rev_ltkey => //.
+  proc; inline.
+  sp; if => //.
+  sp; match = => // st.
+  match = => // sk.
+  if => //.
+  if => //; by auto => />.
+- move => &2 bad.
+  proc; sp; if => //. 
+  match => //.
+  match => //; if; auto => />.
+- move => &1.
+  proc; inline*.
+  rcondf ^if; auto => />.
+
+(* c_rev_ephkey *)
+- conseq (: ={res} /\ ={b0, hm, h1m, h2m, c_smap, s_smap, servers, tested, b_set, x_set, y_set, pk_set, m1_set, m2_set, bad1, bad2, tq, hq, badq, test_ephrev_s, test_ltkrev}(Game4, Game4Eph)) Game4_inv_c_rev_ephkey => //.
+  proc; inline.
+  sp; if => //.
+  sp; match = => // st.
+  match = => // [s pt ir|s t k ir].
+  + auto => />.
+  auto => /> &2 *.
+- move => &2 bad.
+  proc; sp; if => //.
+  match => //.
+  match => //; if => //; auto => /> &hr *.
+- move => &1.
+  proc; inline*.
+  rcondf ^if; auto => />.
+
+(* s_rev_ephkey *) 
+- conseq (: ={res} /\ ={b0, hm, h1m, h2m, c_smap, s_smap, servers, tested, b_set, x_set, y_set, pk_set, m1_set, m2_set, bad1, bad2, tq, hq, badq, test_ephrev_s, test_ltkrev}(Game4, Game4Eph)) Game4_inv_s_rev_ephkey => //.
+- proc; inline.
+  sp; if => //.
+  sp; match = => // st.
+  match = => // s t k ir.
+  if => //; if => //.
+  + auto => |> &2 6?.
+    rewrite negb_and !negb_or.
+    have->: ir.`3 = get_ir_test (oget Game4Eph.s_smap{2}.[b{2}, j{2}]). smt().
+    admit.
+  auto => />.
+- move => &2 bad.
+  proc; sp; if => //.
+  match => //. 
+  match => //.
+  if => //.
+  if => //.
+  auto => />.
+  admit.
+  auto => />.
+- move => &1.
+  proc; inline*.
+  rcondf ^if; auto => />.
+
+(* c_test *)
+- conseq (: ={res} /\ ={b0, hm, h1m, h2m, c_smap, s_smap, servers, tested, b_set, x_set, y_set, pk_set, m1_set, m2_set, bad1, bad2, tq, hq, badq, test_ephrev_s, test_ltkrev}(Game4, Game4Eph)) Game4_inv_c_test => //.
+  proc; inline.
+  sp; if => //.
+  sp; if => //.
+  match = => // => st.
+  match = => // => s t k ir.
+  + if => //.
+    rcondf {1} ^if. auto => />.
+    rcondf {2} ^if. auto => />.
+
+(* I am here *)
+
+    sp 3 3; if {2} => //.
+    + auto => |> &2 18?. 
+      rewrite !negb_or negb_and.
+      move => [#] ? + ? H _ _.
+      rewrite H //=.
+      move => [#] ? ?.
+      rewrite /fresh_partner_c.
+      case (1 <= card (get_partners_c t Game4Ltk.s_smap{2})).
+      + rewrite //=.
+        move => *. split. 
+        + move => *. do split; ~6: smt(mem_set get_setE). 
+          move => i0 b j.
+          case (i0 = i{2}) => ieq; 2: by smt(mem_set get_setE).
+          rewrite !get_setE mem_set ieq //=.
+          case => //.
+          have : card (get_fresh_partners_c t Game4Ltk.s_smap{2} Game4Ltk.servers{2}) <> 0 by smt().
+          rewrite fcard_eq0.
+          move => *.
+          have : (forall x, x \in (get_fresh_partners_c t Game4Ltk.s_smap{2} Game4Ltk.servers{2}) => x = (b, j)).
+          + move => x0.
+            rewrite /get_fresh_partners_c mem_fdom mem_filter /=.
+            move => [#] *. 
+            smt().
+          smt(mem_pick).
+        move => *. do split; ~6: smt(mem_set get_setE). 
+        move => i0 b j.
+        case (i0 = i{2}) => ieq; 2: by smt(mem_set get_setE).
+        rewrite !get_setE mem_set ieq //=.
+        case => //.
+        have : card (get_fresh_partners_c t Game4Ltk.s_smap{2} Game4Ltk.servers{2}) <> 0 by smt().
+        rewrite fcard_eq0.
+        move => *.
+        have : (forall x, x \in (get_fresh_partners_c t Game4Ltk.s_smap{2} Game4Ltk.servers{2}) => x = (b, j)).
+        + move => x0.
+        rewrite /get_fresh_partners_c mem_fdom mem_filter /=.
+          move => [#] *. 
+          smt().
+        smt(mem_pick).
+      rewrite //=.
+      move => *. split. 
+      + move => *. do split; ~6: smt(mem_set get_setE). 
+        move => i0 b j.
+        case (i0 = i{2}) => ieq; 2: by smt(mem_set get_setE).
+        rewrite !get_setE mem_set ieq //=.
+        case => //.
+        move => *.
+        have : (b, j) \in get_partners_c t Game4Ltk.s_smap{2}.
+        + by rewrite /get_partners_c mem_fdom mem_filter /#. search card.
+        have->: (get_partners_c t Game4Ltk.s_smap{2}) = fset0. smt(fcard_eq0 fcard_ge0).
+        by rewrite in_fset0.
+      move => *. do split; ~6: smt(mem_set get_setE). 
+      move => i0 b j.
+      case (i0 = i{2}) => ieq; 2: by smt(mem_set get_setE).
+      rewrite !get_setE mem_set ieq //=.
+      case => //.
+      move => *.
+      have : (b, j) \in get_partners_c t Game4Ltk.s_smap{2}.
+      + by rewrite /get_partners_c mem_fdom mem_filter /#. search card.
+      have->: (get_partners_c t Game4Ltk.s_smap{2}) = fset0. smt(fcard_eq0 fcard_ge0).
+      by rewrite in_fset0.
+    auto => |> &2 18?. 
+    rewrite !negb_or negb_and.
+    move => ? [#] 2? + + ? H.
+    rewrite H //=.
+    move => + H2 ? ? ? ?.
+    rewrite /fresh_partner_c ifT //=. smt(fcard_ge0).
+    rewrite /get_fresh_partners_c.
+    rewrite H //=.
+    move => H3.
+    split. 
+    + have : card (fdom (filter (fun (_ : pkey * int) (val : pr_st_server instance_state) =>
+               get_trace val = Some t /\
+               get_ir_test val = false /\
+               get_ir_sess val = false /\ get_ir_eph val = false) Game4Ltk.s_smap{2})) <> 0 by smt().
+      rewrite fcard_eq0 => /mem_pick /mem_fdom.
+      by rewrite mem_filter /#.
+    do split; 1..3: smt(mem_set get_setE).
+    move => b j bjin []. smt().
+    move => [i0].
+    case (i0 = i{2}) => i0eq; 1: by smt(get_setE mem_set).
+    rewrite mem_set i0eq get_setE i0eq //=.
+    smt().
+  auto => />.
+- move => &2 bad.
+  proc; sp; if => //.
+  rcondf ^if. auto => />.
+  auto => />.
+- move => &1.
+  proc; inline*.
+  rcondf ^if; auto => />.
+
+
+
+
+qed.*)
 
 
 lemma sofar2 &m: `| Pr[E_GAKE_nodhs(GAKEb_nodhs(NTOR_S_mod, NTOR_C_mod, RO), A).run(false) @ &m : res] - Pr[E_GAKE_nodhs(GAKEb_nodhs(NTOR_S_mod, NTOR_C_mod, RO), A).run(true) @ &m : res]|
@@ -4816,7 +5133,7 @@ call (: Game4Ltk.badq,
                       /\ (exists (i j : int), (i \in St_CDH_O.x_map{1}) /\ x.`4 = g ^ oget St_CDH_O.x_map{1}.[i] 
                                /\ x.`1 = x{2}.`5 ^ oget St_CDH_O.x_map{1}.[i] /\ x.`2 = x{2}.`3 ^ oget St_CDH_O.x_map{1}.[i]
                                /\ j \in St_CDH_O.y_map{1} /\ x.`3 = g ^ oget St_CDH_O.y_map{1}.[j] /\ (i \notin St_CDH_O.cr1{1}) /\ (j \notin St_CDH_O.cr2{1})))
-         /\ (forall i, i \in Game4Ltk.c_smap{2} => get_trace (oget Game4Ltk.c_smap{2}.[i]) <> None)
+         /\ (forall i, i \in Game4Ltk.c_smap{2} => get_trace (oget Game4Ltk.c_smap{2}.[i]) <> None /\ (oget (get_trace (oget Game4Ltk.c_smap{2}.[i]))).`1.`2 \in Game4Ltk.m1_set{2})
          /\ (forall b j, (b, j) \in Game4Ltk.s_smap{2} => get_trace (oget Game4Ltk.s_smap{2}.[(b, j)]) <> None)
          /\ (forall b j, (b, j) \in Game4Ltk.s_smap{2} => get_ir_test (oget Game4Ltk.s_smap{2}.[(b, j)]) 
                => (exists i, i \in Game4Ltk.c_smap{2} /\ (oget (get_trace (oget Game4Ltk.s_smap{2}.[(b, j)]))).`1 = (oget (get_trace (oget Game4Ltk.c_smap{2}.[i]))).`1))
@@ -6590,7 +6907,7 @@ smt(get_setE mem_set).
   by auto => />.
 
 (* rev_ltkey *)
-+ proc; inline. admit. (*
++ proc; inline.
   sp; if => //.
   sp; match {1} => //.
   + match None {2} ^match. auto => /#.
@@ -6873,7 +7190,7 @@ smt().
   + match Corrupt_mod {2} ^match. auto => /#.
     auto => />.
   match Dishonest_mod {2} ^match. auto => /#.
-  auto => />. *)
+  auto => />. 
 - move => &2 bad; proc; inline. 
   sp; if => //.
   sp; match => //. 
@@ -7186,7 +7503,7 @@ move => [i2] itr.
 exists i2.
 smt(get_setE mem_set).
   match Aborted_mod {2} ^match. auto => /#.
-  auto => />. 
+  auto => />.
 - move => &2 bad; proc; inline.
   sp; if => //. 
   sp; match => //. 
@@ -7196,7 +7513,8 @@ smt(get_setE mem_set).
   sp; match => //. 
   by match; auto => />.
 
-+ proc; inline.
+(* s_rev_ephkey *)
++ proc; inline. admit. (*
   sp; if => //.
   sp; match {1} => //.
   + match None {2} ^match. auto => /#.
@@ -7343,7 +7661,7 @@ exists i2.
 rewrite bjeq in itr.
 smt(get_setE mem_set).
   match Aborted_mod {2} ^match. auto => /#.
-  auto => />. 
+  auto => />. *)
 - move => &2 bad; proc; inline. 
   sp; if => //.
   sp; match => //. 
@@ -7422,7 +7740,6 @@ smt(get_setE mem_set).
 
 
 
-
 admit.
 move => *. do split; ~1..3,9,10,19,20,23: smt(get_setE mem_set in_fsetU1 loggK expgK expM pow_bij).
 clear inv inv2 inv3 inv4 c1 c2 c3 c4 c5 c6 c7 c8 c9 c10 c11 c12 c13 c14 c15 c16 c17 c18 c19 c20 c21 c22 c23 c24 c25 c26 c27 c28 c29 c30 c31 c32 c33 c34 c35 c36 c37 c38 c39 c40 c41 c42.
@@ -7459,17 +7776,21 @@ move : nltk.
 have->: t'{1}.`1.`1 = t'{2}.`1.`1 by smt().
 clear. smt().
 
-move => x0. 
+move => x0.
 rewrite mem_set //=.
 move => [].
-move => xin x3in x4in i0 i0in x4eq x1eq x2eq.
-rewrite mem_set.
-split. smt().
-have->: st'{2}.`1 = t'{1}.`1.`1. smt().
-have->: g ^ st'{2}.`2 = t'{1}.`1.`2. smt().
-have->: st'{2}.`2 = loge t'{1}.`1.`2. smt(loggK expgK expM). 
-smt(get_setE pow_bij loggK expgK expM).
-admit. admit.
++ move => xin x3in x4in i0 i0in x4eq x1eq x2eq.
+  rewrite mem_set.
+  split. smt().
+  have->: st'{2}.`1 = t'{1}.`1.`1. smt().
+  have->: g ^ st'{2}.`2 = t'{1}.`1.`2. smt().
+  have->: st'{2}.`2 = loge t'{1}.`1.`2. smt(loggK expgK expM). 
+  smt(get_setE pow_bij loggK expgK expM).
+move => -> //=.
+smt(get_setE mem_set loggK expgK expM).
+move => x0.
+rewrite mem_set //=.
+move => []; smt(get_setE mem_set loggK expgK expM).
 move => b0 x0 y0.
 have->: st'{2}.`2 = loge t'{1}.`1.`2. smt(loggK expgK expM). 
 smt(mem_set pow_bij loggK expgK expM).
@@ -7502,12 +7823,8 @@ smt(mem_set pow_bij loggK expgK expM).
 exists (oget Red_Ltk.Red_O.i_inst{1}.[i{2}]) (oget Red_Ltk.Red_O.b_inst{1}.[st'{2}.`1]).
 smt().
 
-
-
-(* I can kill this branch - I know that if x is in h2m then either this instance is tested or session key revealed or its partner is or it has been queried by the adverasry and I have won! *)
-
-
-    auto => /> &1 &2 7? c21 c22 c23 c24 c25 c26 c27 c28 c29 c30 c31 c32 c33 c34 c35 c36 c37 c38 c39 c40 c41 4? c11 c12 c13 c14 c15 c16 c17 c18 c19 c20 c1 c2 c3 c4 c5 c6 c7 c8 inv c9 inv2 c10 inv3 inv4 *. split. 
+    auto => /> &1 &2 7? c21 c22 c23 c24 c25 c26 c27 c28 c29 c30 c31 c32 c33 c34 c35 c36 c37 c38 c39 c40 c41 4? 
+                 c11 c12 c13 c14 c15 c16 c17 c18 c19 c20 c1 c2 c3 c4 c5 c6 c7 c8 inv c9 inv2 c10 inv3 inv4 *. split. 
 admit. (* show that win has happened as above *)
 move => *. do split; ~1,7,8,11: smt(get_setE mem_set in_fsetU1 loggK expgK expM).
 clear inv inv2 inv3 inv4 c1 c2 c3 c4 c5 c6 c7 c8 c9 c10 c11 c12 c13 c14 c15 c16 c17 c18 c19 c20 c21 c22 c23 c24 c25 c26 c27 c28 c29 c30 c31 c32 c33 c34 c35 c36 c37 c38 c39 c40 c41.
@@ -7575,7 +7892,7 @@ simplify.
 move => [#] H1 H2 H3 H H5 H6 H7 H8 H9 *.
 do split; smt(expgK expM loggK).
 
-auto => /> &1 &2 64? ltk *. split.
+auto => /> &1 &2 27? inv 36? ltk *. split.
 have->: (get_fresh_partners_c t'{1} Red_Ltk.Red_O.s_smap{1}
                      Red_Ltk.Red_O.servers{1}) = (get_fresh_partners_c t'{2} Game4Ltk.s_smap{2} Game4Ltk.servers{2}).
 rewrite /get_fresh_partners_c. 
@@ -7603,8 +7920,8 @@ rewrite /get_fresh_partners_c.
         do rewrite mem_fdom mem_filter.
         admit. (* too much in context *)
       smt().
-    smt(get_setE mem_set).
-
+    move : inv. clear.
+    smt().
 move : ltk.
 have->: t'{1}.`1.`1 = t'{2}.`1.`1 by smt().
 smt().
@@ -7653,7 +7970,7 @@ auto => />.
     auto => />.
   + match Accepted_mod {2} ^match. auto => /#.
     if => //.
-    + auto => /> &1 &2 *.
+    + auto => /> &1 &2 24? inv *.
       rewrite /fresh_partner_s.
       rewrite /get_origins_s /get_fresh_partners_s.
       have->: (fdom
@@ -7682,28 +7999,44 @@ auto => />.
         move => x.
         do rewrite mem_fdom mem_filter.
         admit. (* too much in context *)
+      have->: get_ir_sess (oget Red_Ltk.Red_O.s_smap{1}.[b{2}, j{2}]) = get_ir_sess (oget Game4Ltk.s_smap{2}.[b{2}, j{2}]) by smt().
+      have->: get_ir_eph (oget Red_Ltk.Red_O.s_smap{1}.[b{2}, j{2}]) = get_ir_eph (oget Game4Ltk.s_smap{2}.[b{2}, j{2}]) by smt().
+      have->: get_sr_ltk (oget Red_Ltk.Red_O.servers{1}.[b{2}]) = get_sr_ltk (oget Game4Ltk.servers{2}.[b{2}]). 
+      + move : inv. clear. smt().
       smt().
     rcondf {1} ^if. auto => />.
-    rcondf {2} ^if. auto => />.
-    sp; seq 1 1 : (#pre /\ ={ks2}). auto => />.
-    if => //.
-    + auto => /> &1 &2 *. 
-      have->: t'{1} = t'{2}. smt().
-      have<-: st'{1}.`2 = st'{2}.`2. smt().
-      have->: t'{2}.`1.`1 = g ^ st'{2}.`1. smt(). split.
-      smt(get_setE mem_set in_fsetU1 loggK expgK expM).
-      have : g ^ st'{2}.`1 \in Red_Ltk.Red_O.servers{1}. smt().
-      have : t'{2}.`1.`2 \in Game4.m1_set{2}. admit. (* this needs to use freshness condition, since fresh_partner is Some true there is an honest client with this message *)
-      move => *.
-      have : (exists (i : int),
-        (i \in St_CDH_O.x_map{1}) /\
-        t'{2}.`1.`2 = g ^ oget St_CDH_O.x_map{1}.[i] /\
-        t'{2}.`1.`2 ^ oget st'{2}.`2 = g ^ oget st'{2}.`2 ^ oget St_CDH_O.x_map{1}.[i] /\
-        t'{2}.`1.`2 ^ st'{2}.`1 = g ^ st'{2}.`1 ^ oget St_CDH_O.x_map{1}.[i]). smt(get_setE mem_set pow_bij loggK expgK expM ComRing.mulrC).
-      smt(get_setE mem_set loggK expgK expM).
-    + auto => /> &1 &2 49? inv ? inv2 inv3 *. split. 
-     admit. 
-     move => *. do split; ~1,3,4,6,17..19,22: smt(get_setE mem_set in_fsetU1 loggK expgK expM).
+    rcondf {2} ^if. auto => />. 
+    sp; if => //. 
+    + auto => /> &1 &2 25? inv *.
+      move : inv. clear.
+      smt().
+    + sp; seq 1 1 : (#pre /\ ={ks2}). auto => />.
+      if => //.
+      + auto => /> &1 &2 64? fresh nltk *. 
+        have->: t'{1} = t'{2}. smt().
+        have<-: st'{1}.`2 = st'{2}.`2. smt().
+        have->: t'{2}.`1.`1 = g ^ st'{2}.`1. smt(). split.
+        smt(get_setE mem_set in_fsetU1 loggK expgK expM).
+        have : g ^ st'{2}.`1 \in Red_Ltk.Red_O.servers{1}. smt().
+        have : t'{2}.`1.`2 \in Game4Ltk.m1_set{2}. 
+        + move : fresh.
+          rewrite !negb_or negb_and nltk //= => [#] nses.
+          rewrite /fresh_partner_s => fp.
+          have : card (get_fresh_partners_s t'{1} Red_Ltk.Red_O.c_smap{1}) <> 0 by smt().
+          rewrite /get_fresh_partners_s fcard_eq0 => /mem_pick /mem_fdom.
+          rewrite mem_filter /=.
+          move => [H1 H2].
+          smt().
+        move => *.
+        have : (exists (i : int),
+          (i \in St_CDH_O.x_map{1}) /\
+          t'{2}.`1.`2 = g ^ oget St_CDH_O.x_map{1}.[i] /\
+          t'{2}.`1.`2 ^ oget st'{2}.`2 = g ^ oget st'{2}.`2 ^ oget St_CDH_O.x_map{1}.[i] /\
+          t'{2}.`1.`2 ^ st'{2}.`1 = g ^ st'{2}.`1 ^ oget St_CDH_O.x_map{1}.[i]). smt(get_setE mem_set pow_bij loggK expgK expM ComRing.mulrC).
+        smt(get_setE mem_set loggK expgK expM).
+    + auto => /> &1 &2 28? inv4 ? inv7 20? inv ? inv2 inv3 ? inv6 ? inv5 6? fresh nltk *. split. 
+     admit. (* needs the win invariant *)
+     move => *. do split; ~1,3,5,19,20,23,25: smt(get_setE mem_set in_fsetU1 loggK expgK expM).
 have->: (get_fresh_partners_s t'{1} Red_Ltk.Red_O.c_smap{1}) = (get_fresh_partners_s t'{2} Game4Ltk.c_smap{2}).
 rewrite /get_fresh_partners_s.
       have->: (fdom (filter (fun (_ : int) (val : pr_st_client instance_state) =>
@@ -7722,32 +8055,64 @@ rewrite /get_fresh_partners_s.
         admit. (* too much in context *)
       smt().
 smt().
+move : inv4 nltk. clear. smt().
 move => x0.
-rewrite mem_set.
-move => []. 
+case (x0 = (t'{2}.`1.`2 ^ oget st'{2}.`2, t'{2}.`1.`2 ^ st'{2}.`1, g ^ st'{2}.`1, t'{2}.`1.`2, g ^ oget st'{2}.`2)).
++ move => -> //= *. 
+  have : t'{2}.`1.`2 \in Game4Ltk.m1_set{2}.
+  + move : fresh.
+    rewrite !negb_or negb_and nltk //= => [#] nses.
+    rewrite /fresh_partner_s => fp.
+    have : card (get_fresh_partners_s t'{1} Red_Ltk.Red_O.c_smap{1}) <> 0 by smt().
+    rewrite /get_fresh_partners_s fcard_eq0 => /mem_pick /mem_fdom.
+    rewrite mem_filter /=.
+    move => [#] H1 [m2] H2 H3 H4 H5.
+    have := inv6 (pick
+   (fdom
+      (filter
+         (fun (_ : int) (val : pr_st_client instance_state) =>
+            (exists (m2o : (pkey * tag) option),
+               get_trace val = Some (t'{1}.`1, m2o)) /\
+            get_ir_test val = false /\
+            get_ir_sess val = false /\ get_ir_eph val = false) Red_Ltk.Red_O.c_smap{1}))).
+    have->: (pick
+   (fdom
+      (filter
+         (fun (_ : int) (val : pr_st_client instance_state) =>
+            (exists (m2o : (pkey * tag) option),
+               get_trace val = Some (t'{1}.`1, m2o)) /\
+            get_ir_test val = false /\
+            get_ir_sess val = false /\ get_ir_eph val = false) Red_Ltk.Red_O.c_smap{1})) \in Game4Ltk.c_smap{2}) by smt().
+    have->: (get_trace
+        (oget
+           Game4Ltk.c_smap{2}.[pick
+                        (fdom
+                           (filter
+                              (fun (_ : int)
+                                 (val : pr_st_client instance_state) =>
+                                 (exists (m2o : (pkey * tag) option),
+                                    get_trace val = Some (t'{1}.`1, m2o)) /\
+                                 get_ir_test val = false /\
+                                 get_ir_sess val = false /\
+                                 get_ir_eph val = false) Red_Ltk.Red_O.c_smap{1}))])) = get_trace
+      (oget
+         Red_Ltk.Red_O.c_smap{1}.[pick
+                      (fdom
+                         (filter
+                            (fun (_ : int)
+                               (val : pr_st_client instance_state) =>
+                               (exists (m2o : (pkey * tag) option),
+                                  get_trace val = Some (t'{1}.`1, m2o)) /\
+                               get_ir_test val = false /\
+                               get_ir_sess val = false /\
+                               get_ir_eph val = false) Red_Ltk.Red_O.c_smap{1}))]). move : inv7. clear. smt().
+    smt().
+  smt().
 move => *.
 have->: t'{1} = t'{2}. smt().
 have<-: st'{1}.`2 = st'{2}.`2. smt().
 have->: t'{2}.`1.`1 = g ^ st'{2}.`1. smt().
-split. smt(get_setE mem_set in_fsetU1 loggK expgK expM).
 smt(get_setE mem_set in_fsetU1 loggK expgK expM).
-move => -> //= *. 
-have->: t'{1} = t'{2}. smt().
-have<-: st'{1}.`2 = st'{2}.`2. smt().
-have->: t'{2}.`1.`1 = g ^ st'{2}.`1. smt().
-split. smt(get_setE mem_set in_fsetU1 loggK expgK expM).
-smt(get_setE mem_set in_fsetU1 loggK expgK expM).
-move => x0.
-have : t'{2}.`1.`2 \in Game4.m1_set{2}. admit.
-smt(get_setE mem_set in_fsetU1 loggK expgK expM).
-move => x0.
-have : t'{2}.`1.`2 \in Game4.m1_set{2}. admit.
-smt(get_setE mem_set in_fsetU1 loggK expgK expM).
-move => i t1 t2.
-case : (i = (b, j){2}); 2: by smt(get_setE).
-move => -> //=.
-have := inv (b, j){2} t1 t2.
-smt(get_setE).
 + move => // i0 i'.
         case (i0 = (b, j){2}) => ieq.
         + rewrite ieq get_set_sameE //=.
@@ -7779,6 +8144,10 @@ exists (oget Red_Ltk.Red_O.i_inst{1}.[]) (oget Red_Ltk.Red_O.b_inst{1}.[(b, j){2
 do split; 1..7: smt().
 admit. (* connect with freshness condition as in corruption *)*)
 
+move => b0 j0.
+case ((b0, j0) = (b, j){2}) => bjeq; 2: by smt(get_setE mem_set).
+rewrite mem_set get_setE bjeq //=.
+admit. (* I also need to extract partner instance here *)
 
 
     auto => /> &1 &2 49? inv ? inv2 inv3 *. split. 
@@ -7854,101 +8223,6 @@ admit. (* connect with freshness condition as in corruption *)*)
   match; auto => />.
   by if => //; if => //; auto => />; rewrite dkey_ll.
 qed.
-
-module Reduction_Eph (A : A_GAKE_nodhs) (D : DDH_oracle) = {
-  var solution : group option
-
-  module Red_O : GAKE_nodhs_i = GameDDH with {
-    var t_i, t_j : int
-    var t_b : pkey
-    var ga, gb : group
-    var stop : bool
-
-    proc init_mem [
-      -1 + {stop <- false; t_b <- witness;}
-    ]
-
-    proc h [
-       0 + ^ {rt <- witness; rk <- witness; }
-      [0 - ^rk<-] + ^ (!stop)
-      ^t<$ + ^ {stop <- stop \/ ((x1, x2) = (None, None));}
-    ]
-
-    proc init_s [
-      [0 - ^if] + ^ (!stop)
-    ]
-
-    proc send_msg1 [
-      [0 - ^if] + ^ (!stop)
-      ^if.^match#None.^if.^pk<- + ^ (i = t_i)
-      ^if.^match#None.^if.^kp_set<- + {pk <- ga; t_b <- m1;}
-    ]
-
-    proc send_msg2 [
-      [0 - ^match] + ^ (!stop)
-      ^match#Some.^match#None.^if.^pk<- + ^ (b = t_b /\ j = t_j)
-      ^match#Some.^match#None.^if.^kp_set<- + {pk <- gb;}
-    ]
-
-    proc send_msg3 [
-      [0 - ^match] + ^ (!stop)
-    ]
-
-    proc c_rev_skey [
-      [0 - ^match] + ^ (!stop)
-    ]
-
-    proc s_rev_skey [
-      [0 - ^match] + ^ (!stop)
-    ]
-
-    proc rev_ltkey [
-      [0 - ^match] + ^ (!stop)
-    ]
-
-    proc c_rev_ephkey [
-      [0 - ^match] + ^ (!stop)
-    ]
-
-    proc s_rev_ephkey [
-      [0 - ^match] + ^ (!stop)
-    ]
-
-    proc c_test [
-      [0 - ^if] + ^ (!stop)
-    ]
-
-    proc s_test [
-      [0 - ^if] + ^ (!stop)
-    ]
-
-  }
-
-  proc solve(t_i, t_j : int, ga, gb : group) : group option = {
-    var b' : bool;
-
-    solution <- witness;
-    Red_O.t_i <- t_i;
-    Red_O.t_j <- t_j;
-    Red_O.ga <- ga;
-    Red_O.gb <- gb;
-    b' <@ A(Red_O).run();
-    return solution;
-  }
-}.
-
-print Reduction_Eph.Red_O.
-
-
-lemma embed_eph &m i j: `| Pr[GAKEc.E_GAKE_nodhs(GAKEb_st(NTOR_S(GAKEc.HROc.RO), NTOR_C(GAKEc.HROc.RO), GAKEc.HROc.RO), Hon_s_Red(A)).run(bit) @ &m : res]
-     - Pr[GAKE_mod.E_GAKE_nodhs(GAKE_mod.GAKEb_nodhs(NTOR_S_mod(GAKE_mod.HROc.RO), NTOR_C_mod(GAKE_mod.HROc.RO), GAKE_mod.HROc.RO), Name_Red(Hon_s_Red(A))).run(bit) @ &m : res] | 
-                 <= Pr[GAKEc.E_GAKE_nodhs(GAKEb_st(NTOR_S(GAKEc.HROc.RO), NTOR_C(GAKEc.HROc.RO), GAKEc.HROc.RO), Hon_s_Red(A)).run(bit) @ &m : GAKEb_st.stop].
-proof.
-rewrite StdOrder.RealOrder.distrC.
-byequiv (: _ ==> _) : Name_Red.O_GAKE.stop => //; first last.
-+ smt().
-symmetry; proc; inline*.
-wp; call (: Name_Red.O_GAKE.stop
 
 
 end section.
